Added failing test for nested subset types

Test/git-issues/git-issue-1604d.dfy
@@ -54,6 +54,24 @@ function method {:opaque} getOriginalSet(): set<Cell> {
 predicate method isSetOfGhostOrdinalCells(s: set<GhostOrdinalCell>) {
   forall c :: c in s ==> returnsOneIfGhostOrdinalCell(c) == 1
 }
-predicate method isSetOfCompilableEvenCells(s: set<CompilableOrdinalCell>) {
+predicate method isSetOfCompilableOrdinalCells(s: set<CompilableOrdinalCell>) {
   forall c :: c in s ==> returnsOneIfCompilableOrdinalCell(c) == 1
+}
+
+method Main() {
+  var x: set<Cell> := getOriginalSet();
+  // TODO: Test that the following case correctly compile:
+  var b := true;
+
+  // This line should work because c should be of type Cell as the constraint is not compilable
+  // Since it figures out the type of c later, it will be resolved as a "GhostEvenCell" everywhere.
+  b := b && isSetOfGhostOrdinalCells(set c | c in x && c.x >= 1 && ghostOrdinalCellIsOneOrMore(c) :: c);
+
+  b := b && isSetOfCompilableOrdinalCells(set c: CompilableOrdinalCell | c in x && compiledOrdinalCellIsOneOrMore(c) :: c);
+
+  /** The following should fail
+  b := b && isSetOfCompilableOrdinalCells(set c: GhostOrdinalCell | c in x && ghostOrdinalCellIsOneOrMore(c) :: c);
+  b := b && isSetOfCompilableOrdinalCells(set c: GhostOrdinalCell2 | c in x && ghostOrdinalCellIsOneOrMore(c) :: c);
+  b := b && isSetOfCompilableOrdinalCells(set c: GhostOrdinalCell3| c in x && ghostOrdinalCellIsOneOrMore(c) :: c);
+  */
 }
